Coq Developments/msci/Metatheory/MetatheoryAtom.v
@@ -123,6 +123,8 @@ Module Import AtomSetImpl : FSetExtra.WSfun AtomDT :=
 Notation atoms :=
   AtomSetImpl.t.
 
+Notation elems := AtomSetImpl.elements.
+
 (** The [AtomSetDecide] module provides the [fsetdec] tactic for
     solving facts about finite sets of atoms. *)
 
